Remove State.Nontrivial type class and factor it out a la State.Trivial
Bump Lean and Mathlib

src/ReactorModel/Determinism/ExecutionStep.lean
@@ -5,16 +5,9 @@ namespace Execution
 open ReactorType
 open State (Closed)
 
-variable [Practical α] {s s₁ s₂ : State α} [State.Nontrivial s] [State.Nontrivial s₁] in section
+variable [Practical α] {s s₁ s₂ : State α}
 
 namespace AdvanceTag
-
-theorem not_closed (a : s₁ ⇓- s₂) : ¬(Closed s₂) :=
-  have := a.advance.preserves_nontrivial -- TODO: Make this work via type class inference.
-  (·.progress_Nonempty.ne_empty a.advance.progress_empty)
-
-theorem nonrepeatable (a₁ : s₁ ⇓- s₂) (a₂ : s₂ ⇓- s₃) : False :=
-  a₁.not_closed a₂.closed
 
 theorem tag_lt (a : s₁ ⇓- s₂) : s₁.tag < s₂.tag :=
   a.advance.tag_lt
@@ -25,9 +18,6 @@ theorem tag_ne (a : s₁ ⇓- s₂) : s₁.tag ≠ s₂.tag :=
 theorem deterministic (a₁ : s ⇓- s₁) (a₂ : s ⇓- s₂) : s₁ = s₂ :=
   a₁.advance.deterministic a₂.advance
 
-instance preserves_nontrivial [State.Nontrivial s₁] {e : s₁ ⇓- s₂} : State.Nontrivial s₂ :=
-  e.advance.preserves_nontrivial
-
 end AdvanceTag
 
 namespace Instantaneous
@@ -35,6 +25,9 @@ namespace ClosedExecution
 
 theorem not_closed (e : s₁ ⇓| s₂) : ¬s₁.Closed := 
   e.exec.not_closed
+
+theorem nonrepeatable (e₁ : s₁ ⇓| s₂) (e₂ : s₂ ⇓| s₃) : False :=
+  e₂.not_closed e₁.closed
 
 theorem acyclic (e : s₁ ⇓| s₂) (h : rcn ∈ e.rcns) : rcn ≮[s₁.rtr] rcn :=
   e.exec.acyclic h
@@ -45,7 +38,7 @@ theorem preserves_tag (e : s₁ ⇓| s₂) : s₁.tag = s₂.tag :=
 theorem equiv (e : s₁ ⇓| s₂) : s₁.rtr ≈ s₂.rtr :=
   e.exec.equiv
   
-theorem rcns_Nodup (e : s₁ ⇓| s₂) : e.rcns.Nodup := 
+theorem rcns_nodup (e : s₁ ⇓| s₂) : e.rcns.Nodup := 
   e.exec.rcns_nodup
 
 theorem progress_def (e : s₁ ⇓| s₂) : s₂.progress = s₁.rtr[.rcn].ids :=
@@ -59,7 +52,7 @@ theorem progress_empty_mem_rcns_iff (e : s₁ ⇓| s₂) (h : s₁.progress = �
   simp [e.mem_rcns_iff, h]
 
 theorem rcns_perm (e₁ : s ⇓| s₁) (e₂ : s ⇓| s₂) : e₁.rcns ~ e₂.rcns := by
-  simp [List.perm_ext e₁.rcns_Nodup e₂.rcns_Nodup, e₁.mem_rcns_iff, e₂.mem_rcns_iff]
+  simp [List.perm_ext e₁.rcns_nodup e₂.rcns_nodup, e₁.mem_rcns_iff, e₂.mem_rcns_iff]
 
 theorem tag_eq (e₁ : s ⇓| s₁) (e₂ : s ⇓| s₂) : s₁.tag = s₂.tag :=
   e₁.exec.preserves_tag ▸ e₂.exec.preserves_tag
@@ -70,14 +63,11 @@ theorem progress_eq (e₁ : s ⇓| s₁) (e₂ : s ⇓| s₂) : s₁.progress = 
 theorem step_determined (e : s ⇓| s₁) (a : s ⇓- s₂) : False :=
   e.not_closed a.closed
 
-instance preserves_nontrivial [h : State.Nontrivial s₁] {e : s₁ ⇓| s₂} : State.Nontrivial s₂ where
-  nontrivial := Equivalent.obj?_rcn_eq e.equiv ▸ h.nontrivial
-
-theorem nonrepeatable (e₁ : s₁ ⇓| s₂) (e₂ : s₂ ⇓| s₃) : False :=
-  e₂.not_closed e₁.closed
-
 theorem progress_ssubset (e : s₁ ⇓| s₂) : s₁.progress ⊂ s₂.progress :=
   e.exec.progress_ssubset
+
+theorem deterministic (e₁ : s ⇓| s₁) (e₂ : s ⇓| s₂) : s₁ = s₂ :=
+  e₁.exec.deterministic e₂.exec (e₁.tag_eq e₂) (e₁.progress_eq e₂)
 
 end ClosedExecution
 end Instantaneous
@@ -88,32 +78,14 @@ theorem tag_le : (s₁ ⇓ s₂) → s₁.tag ≤ s₂.tag
   | close e   => le_of_eq e.preserves_tag
   | advance a => le_of_lt a.tag_lt
 
-theorem seq_tag_lt : (s₁ ⇓ s₂) → (s₂ ⇓ s₃) → s₁.tag < s₃.tag
-  | close e₁,   close e₂   => e₁.nonrepeatable e₂ |>.elim
-  | advance a₁, advance a₂ => a₁.nonrepeatable a₂ |>.elim
-  | close e,    advance a  => e.preserves_tag ▸ a.tag_lt
-  | advance a,  close e    => e.preserves_tag ▸ a.tag_lt
-
-instance preserves_nontrivial [State.Nontrivial s₁] : (s₁ ⇓ s₂) → State.Nontrivial s₂
-  | close e   => e.preserves_nontrivial
-  | advance a => a.preserves_nontrivial
-
 theorem resolve_close : (e : s₁ ⇓ s₂) → ¬s₁.Closed → Nonempty (s₁ ⇓| s₂)
   | close e  , _ => ⟨e⟩
   | advance a, h => absurd a.closed h
 
-end Step
-
-end
-
-variable [Practical α] {s s₁ s₂ : State α}
-
-theorem Instantaneous.ClosedExecution.deterministic (e₁ : s ⇓| s₁) (e₂ : s ⇓| s₂) : s₁ = s₂ :=
-  e₁.exec.deterministic e₂.exec (e₁.tag_eq e₂) (e₁.progress_eq e₂)
-
-theorem Step.deterministic : (s ⇓ s₁) → (s ⇓ s₂) → s₁ = s₂
+theorem deterministic : (s ⇓ s₁) → (s ⇓ s₂) → s₁ = s₂
   | close e₁, close e₂                      => e₁.deterministic e₂
   | advance a₁, advance a₂                  => a₁.deterministic a₂
   | close e, advance a | advance a, close e => e.step_determined a |>.elim
 
+end Step
 end Execution
