src/ReactorModel.lean
@@ -1,5 +1,5 @@
-import ReactorModel.Objects
 import ReactorModel.Determinism
 import ReactorModel.Execution
 import ReactorModel.Extensions
+import ReactorModel.Objects
 import ReactorModel.Primitives
