src/ReactorModel/Determinism/Execution.lean
@@ -1,5 +1,5 @@
-import ReactorModel.Determinism.ExecutionStep
-import ReactorModel.Determinism.Trivial
+import ReactorModel.Determinism.Trivial 
+import ReactorModel.Determinism.Nontrivial
 
 open Classical
 
@@ -7,37 +7,11 @@ namespace Execution
 
 variable [ReactorType.Practical α] {s s₁ s₂ : State α}
 
-theorem tag_le {s₁ s₂ : State α} (e : s₁ ⇓* s₂) : s₁.tag ≤ s₂.tag := by
-  induction e with
-  | refl        => exact le_refl _
-  | step e _ hi => exact le_trans e.tag_le hi
-
-theorem seq_progress_ssubset_or_tag_lt [State.Nontrivial s₁] : 
-    (s₁ ⇓ s₂) → (s₂ ⇓* s₃) → (s₁.progress ⊂ s₃.progress) ∨ (s₁.tag < s₃.tag)
-  | e₁₂,        step e e' => .inr $ lt_of_lt_of_le (e₁₂.seq_tag_lt e) e'.tag_le
-  | .close e,   refl      => .inl $ e.progress_ssubset
-  | .advance a, refl      => .inr $ a.tag_lt
-
-theorem nontrivial_deterministic {s s₁ s₂ : State α} [nontriv : State.Nontrivial s]
-    (e₁ : s ⇓* s₁) (e₂ : s ⇓* s₂) (ht : s₁.tag = s₂.tag) (hp : s₁.progress = s₂.progress) : 
-    s₁ = s₂ := by
-  induction e₁ generalizing s₂ nontriv <;> cases e₂
-  case refl.refl => rfl
-  case step.step e₁ _ hi _ e₂ e₂' =>
-    have := e₁.preserves_nontrivial -- TODO: Make this work via type class inference.
-    exact hi (e₁.deterministic e₂ ▸ e₂') ht hp
-  all_goals
-    have e := ‹_ ⇓ _›; have e' := ‹_ ⇓* _›
-    have := e.preserves_nontrivial
-    exact match seq_progress_ssubset_or_tag_lt e e' with
-    | .inl h => absurd hp (Set.ssubset_ne $ by simp_all) 
-    | .inr h => absurd ht $ ne_of_lt (by simp_all)
-
 -- TODO: This theorem can be proven over non-`Finite` but `LawfulUpdatable`, `Proper` reactors. 
 theorem deterministic : 
     (s ⇓* s₁) → (s ⇓* s₂) → (s₁.tag = s₂.tag) → (s₁.progress = s₂.progress) → s₁ = s₂ := 
-  if h : State.Nontrivial s 
-  then nontrivial_deterministic
+  if h : s.Nontrivial 
+  then nontrivial_deterministic h
   else fun e₁ e₂ ht _ => e₁.trivial_deterministic h e₂ ht
   
 end Execution
