src/ReactorModel/Determinism/Nontrivial.lean
@@ -1,0 +1,82 @@
+import ReactorModel.Determinism.ExecutionStep
+
+open ReactorType Classical
+
+namespace Execution
+
+variable [Practical α] {s s₁ s₂ : State α}
+
+namespace State
+
+def Nontrivial (s : State α) : Prop :=
+  s.rtr[.rcn].Nonempty
+
+theorem Nontrivial.equiv (e : s₁.rtr ≈ s₂.rtr) (n : s₁.Nontrivial) : s₂.Nontrivial := by
+  simp_all [Nontrivial, Equivalent.obj?_rcn_eq e]
+
+theorem Closed.progress_nonempty (n : s.Nontrivial) (h : Closed s) : s.progress.Nonempty := by
+  simp_all [Closed, ←Partial.Nonempty.iff_ids_nonempty]
+  exact n
+
+theorem Advance.preserves_nontrivial (n : Nontrivial s₁) : (Advance s₁ s₂) → s₂.Nontrivial
+  | ⟨_, c⟩ => n.equiv c.equiv
+
+end State
+
+namespace AdvanceTag
+
+theorem not_closed (a : s₁ ⇓- s₂) (n : s₁.Nontrivial) : ¬s₂.Closed :=
+  (·.progress_nonempty (a.advance.preserves_nontrivial n) |>.ne_empty a.advance.progress_empty)
+
+theorem nonrepeatable (a₁ : s₁ ⇓- s₂) (a₂ : s₂ ⇓- s₃) (n : s₁.Nontrivial) : False :=
+  a₁.not_closed n a₂.closed
+
+instance preserves_nontrivial {e : s₁ ⇓- s₂} (n : s₁.Nontrivial) : s₂.Nontrivial :=
+  e.advance.preserves_nontrivial n
+
+end AdvanceTag
+
+theorem Instantaneous.ClosedExecution.preserves_nontrivial {e : s₁ ⇓| s₂} (n : s₁.Nontrivial) : 
+    s₂.Nontrivial := by
+  simp_all [State.Nontrivial, Equivalent.obj?_rcn_eq e.equiv]
+
+namespace Step
+
+theorem seq_tag_lt (n : s₁.Nontrivial) : (s₁ ⇓ s₂) → (s₂ ⇓ s₃) → s₁.tag < s₃.tag
+  | close e₁,   close e₂   => e₁.nonrepeatable e₂ |>.elim
+  | advance a₁, advance a₂ => a₁.nonrepeatable a₂ n |>.elim
+  | close e,    advance a  => e.preserves_tag ▸ a.tag_lt
+  | advance a,  close e    => e.preserves_tag ▸ a.tag_lt
+
+instance preserves_nontrivial (n : s₁.Nontrivial) : (s₁ ⇓ s₂) → s₂.Nontrivial
+  | close e   => e.preserves_nontrivial n
+  | advance a => a.preserves_nontrivial n
+
+end Step
+
+-- TODO: This doesn't require nontrivial.
+theorem tag_le {s₁ s₂ : State α} (e : s₁ ⇓* s₂) : s₁.tag ≤ s₂.tag := by
+  induction e with
+  | refl        => exact le_refl _
+  | step e _ hi => exact le_trans e.tag_le hi
+
+theorem seq_progress_ssubset_or_tag_lt (n : s₁.Nontrivial) : 
+    (s₁ ⇓ s₂) → (s₂ ⇓* s₃) → (s₁.progress ⊂ s₃.progress) ∨ (s₁.tag < s₃.tag)
+  | e₁₂,        step e e' => .inr $ lt_of_lt_of_le (e₁₂.seq_tag_lt n e) e'.tag_le
+  | .close e,   refl      => .inl $ e.progress_ssubset
+  | .advance a, refl      => .inr $ a.tag_lt
+
+theorem nontrivial_deterministic {s s₁ s₂ : State α} (n : s.Nontrivial)
+    (e₁ : s ⇓* s₁) (e₂ : s ⇓* s₂) (ht : s₁.tag = s₂.tag) (hp : s₁.progress = s₂.progress) : 
+    s₁ = s₂ := by
+  induction e₁ generalizing s₂ <;> cases e₂
+  case refl.refl => rfl
+  case step.step e₁ _ hi _ e₂ e₂' =>
+    exact hi (e₁.preserves_nontrivial n) (e₁.deterministic e₂ ▸ e₂') ht hp
+  all_goals
+    have e := ‹_ ⇓ _›; have e' := ‹_ ⇓* _›
+    exact match seq_progress_ssubset_or_tag_lt n e e' with
+    | .inl h => absurd hp (Set.ssubset_ne $ by simp_all) 
+    | .inr h => absurd ht $ ne_of_lt (by simp_all)
+
+end Execution
